---
layout:  post
title:   Lab 5
tagline: CNF Conversion

buttonNames: ['Example 1', 'Example 2']
buttonLinks: ['#io', '#another-grammar']
---

## Goal

Transform a [Context-free grammar](https://en.wikipedia.org/wiki/Context-free_grammar) into its Chomsky Normal Form (CNF) — ie: having its productions in on of these forms:

- $A \rightarrow BC$ 
- $A \rightarrow x$

where $A, B, C​$ are variables and $x​$ is a letter. This means productions like $A \rightarrow BCD​$ or $A \rightarrow xC​$ will need to be converted.

We will do this conversion in 4 steps. Each step will be illustrated on the following grammar:
$$
\begin{align}
S & \rightarrow XXY\ |\ Y\ |\ a \\
X & \rightarrow S\ |\ c\ |\ \lambda \\
Y & \rightarrow XY\ |\ Yb\ |\ a\ |\ b
\end{align}
$$

## Step 1 — remove null productions

A variable $V$ is **nullable** if there is a production $V \rightarrow \lambda$ or there is a derivation that starts with $V$ and ends in $\lambda$, ie: $V \rightarrow^* \lambda$.

This is done in 4 sub-steps:

1. Mark every $N$ as nullable if there is a production $N \rightarrow \lambda$
2. Mark every $V$ as nullable if there is a production $V \rightarrow N$ where $N$ is already nullable. Repeat this step until no more nullable variables are marked.
3. For each production $V \rightarrow \alpha$, add to the grammar all productions $V \rightarrow \alpha'$ where $\alpha'$ is obtained from $\alpha$ by removing one or more nullable variables. Eg: $V \rightarrow NM$ (where $N$ and $M$ are nullable) will add $V \rightarrow N$ (removed the $M$), $V \rightarrow M$ (removed the $N$)
4. Remove all $\lambda$-productions $V \rightarrow \lambda$

### Example

In our grammar, the only nullable state is $X$ (because of the production $X \rightarrow \lambda$).

We will add the productions:

- $S \rightarrow XY$, because we had $S \rightarrow XXY$
- $S \rightarrow Y$ already existed
- $Y \rightarrow Y$, because we had $Y \rightarrow XY$

Finally, we remove the $\lambda$-production $X \rightarrow \lambda$.

That means our grammar now looks like this:


$$
\begin{align}
S & \rightarrow XXY\ |\ Y\ |\ a\ |\ XY \\
X & \rightarrow S\ |\ a\ \\
Y & \rightarrow XY\ |\ Yb\ |\ a\ |\ b\ |\ Y
\end{align}
$$


## Step 2 — remove renaming productions

Instead of having the productions:

- $V \rightarrow W$
- $W \rightarrow \alpha$ (anything having $W$ on the left-hand-side)

we add the productions $V \rightarrow \alpha$. That is, directly derive $V$ into anything that $W$ can derive, instead of just renaming $V$ into $W$.

### Example

In our grammar, for the renaming production is $S \rightarrow Y$, because $Y$ has the following productions: 

- $Y  \rightarrow XY$
- $Y  \rightarrow Yb$
- $Y  \rightarrow a$
- $Y  \rightarrow b$


we add the productions:

- $S  \rightarrow XY$ (already existed)
- $S  \rightarrow Yb$
- $S  \rightarrow a$ (already existed)
- $S  \rightarrow b$


For the renaming production $X \rightarrow S$, because  $S$ has the following productions:

- $S  \rightarrow XXY$
- $S  \rightarrow a$
- $S  \rightarrow XY$
- $S  \rightarrow Yb$ (added previously)
- $S  \rightarrow b$ (added previously)

we add the productions:

- $X  \rightarrow XXY$
- $X  \rightarrow a$
- $X  \rightarrow XY$
- $X  \rightarrow Yb$
- $X  \rightarrow b$


The last renaming production $Y \rightarrow Y$ is trivial and can be simply removed.

Our grammar now looks like this:


$$
\begin{align}
S & \rightarrow XXY\ |\ a\ |\ XY\ |\ Yb\ |\ b \\
X & \rightarrow XXY\ |\ a\ |\ XY\ |\ Yb\ |\ b\ |\ c \\
Y & \rightarrow XY\ |\ Yb\ |\ a\ |\ b
\end{align}
$$

## Step 3 — replace long productions

Replace any production $V \rightarrow \alpha_1 \alpha_2 ... \alpha_n$, where $n > 2$ with:

- $V \rightarrow \alpha_1 W$ (the variable $W$ is a new one that did not exist in the grammar)
- $W \rightarrow \alpha_2 ... \alpha_n$

Repeat until there are no productions with more than two symbols (variables or letters) on the right-hand-side.

### Example

In our grammar, for the production $S \rightarrow XXY$, we chose an unused variable $Z$ and add the productions:

- $S \rightarrow XZ$
- $Z \rightarrow XY$

Same for the production $X \rightarrow XXY$: replace it with $X \rightarrow XZ$

Our grammar now looks like this:


$$
\begin{align}
S & \rightarrow XZ\ |\ a\ |\ XY\ |\ Yb\ |\ b \\
X & \rightarrow XZ\ |\ a\ |\ XY\ |\ Yb\ |\ b\ |\ c \\
Y & \rightarrow XY\ |\ Yb\ |\ a\ |\ b \\
Z & \rightarrow XY
\end{align}
$$

> *Note*: if we had a production $S \rightarrow Xab$, it would get replaced in the same manner: $S \rightarrow Tb$ and $T \rightarrow Xa$.
>
> If we had even longer productions: $A \rightarrow abcd$, we would add $A \rightarrow aB$, then $B \rightarrow bC$ and $C \rightarrow cd$.

## Step 4 — replace combined right-hand-sides

Replace every production in the form of:

- $V \rightarrow xW$  or 
- $V \rightarrow Wx$ 

with the productions:
- $V \rightarrow V_xW$  or 
- $V \rightarrow WV_x$ 

where $V_x$ is a new variable with its sole production $V_x \rightarrow x$.

### Example

In our grammar, the productios combining variables and letters on the right-hand-side are:

- $S \rightarrow Yb$. 
- $X \rightarrow Yb$. 
- $Y \rightarrow Yb$. 


We create a new variable $B$ and add the productions:

- $B \rightarrow b$
- $S \rightarrow YB$
- $X \rightarrow YB$
- $Y \rightarrow YB$

The final grammar looks like this:


$$
\begin{align}
S & \rightarrow XZ\ |\ a\ |\ XY\ |\ YB\ |\ b \\
X & \rightarrow XZ\ |\ a\ |\ XY\ |\ YB\ |\ b\ |\ c \\
Y & \rightarrow XY\ |\ YB\ |\ a\ |\ b \\
Z & \rightarrow XY \\
B & \rightarrow b
\end{align}
$$

## IO

<details markdown="1"><summary>Input <code>Grammar.in</code></summary>

Each row contains one production.  `_` stands for $\lambda$. 

```
S -> XXY | Y | a
X -> S | c | _
Y -> XY | Yb | a | b
```

</details>

<details markdown="1"><summary>Output <code>Grammar.out</code> in CNF</summary>

```
S -> XY | YB | a | b | XZ
X -> XY | YB | a | b | XZ | c
Y -> XY | YB | a | b
Z -> XY
B -> b
```

</details>



## Another grammar

<details markdown="1"><summary>Input <code>Grammar.in</code></summary>

Each row contains one production.  `_` stands for $\lambda$. 

```
S -> aX | Yb
X -> S | _
Y -> bY | b
```

</details>

<details markdown="1"><summary>Output <code>Grammar.out</code> in CNF</summary>

Solving steps can be found [here](https://youtu.be/q0HAqPeqwvs).

```
S -> AX | a | YB
X -> AX | a | YB
Y -> BY | b
A -> a
B -> b
```

</details>